iris/SpecFilestat.v
@@ -225,7 +225,7 @@ Record fstat_names := MkFStatNames {
 Global Instance fstat_names_inhabited : Inhabited fstat_names :=
   populate (MkFStatNames
     (UartNames 1%positive 1%positive 1%positive 1%positive)
-    (DiskNames 1%positive 1%positive 1%positive 1%positive 1%positive
+    (DiskNames 1%positive 1%positive 1%positive 1%positive 1%positive 1%positive
                1%positive 1%positive)
     1%positive
     (mword_of_int 0) (mword_of_int 0) (mword_of_int 0)
